doc/book/code/Part1.Quicksort.Generic.fst
@@ -1,0 +1,115 @@
+module Part1.Quicksort.Generic
+
+//Some auxiliary definitions to make this a standalone example
+let rec length #a (l:list a)
+  : nat
+  = match l with
+    | [] -> 0
+    | _ :: tl -> 1 + length tl
+
+let rec append #a (l1 l2:list a)
+  : list a
+  = match l1 with
+    | [] -> l2
+    | hd :: tl -> hd :: append tl l2
+
+let total_order (#a:Type) (f: (a -> a -> bool)) =
+    (forall a. f a a)                                         (* reflexivity   *)
+    /\ (forall a1 a2. (f a1 a2 /\ a1=!=a2)  <==> not (f a2 a1))  (* anti-symmetry *)
+    /\ (forall a1 a2 a3. f a1 a2 /\ f a2 a3 ==> f a1 a3)        (* transitivity  *)
+    /\ (forall a1 a2. f a1 a2 \/ f a2 a1)                       (* totality *)
+
+let total_order_t (a:Type) = f:(a -> a -> bool) { total_order f }
+
+let rec sorted #a  (f:total_order_t a) (l:list a)
+  : bool
+  = match l with
+    | [] -> true
+    | [x] -> true
+    | x :: y :: xs -> f x y && sorted f (y :: xs)
+
+let rec mem (#a:eqtype) (i:a) (l:list a)
+  : bool
+  = match l with
+    | [] -> false
+    | hd :: tl -> hd = i || mem i tl
+
+let rec partition (#a:Type) (f:a -> bool) (l:list a)
+  : x:(list a & list a) { length (fst x) + length (snd x) = length l }
+  = match l with
+    | [] -> [], []
+    | hd::tl ->
+      let l1, l2 = partition f tl in
+      if f hd
+      then hd::l1, l2
+      else l1, hd::l2
+
+let rec sort #a (f:total_order_t a) (l:list a)
+  : Tot (list a) (decreases (length l))
+  = match l with
+    | [] -> []
+    | pivot :: tl ->
+      let hi, lo  = partition (f pivot) tl in
+      append (sort f lo) (pivot :: sort f hi)
+
+
+let rec partition_mem (#a:eqtype)
+                      (f:(a -> bool))
+                      (l:list a)
+  : Lemma (let l1, l2 = partition f l in
+           (forall x. mem x l1 ==> f x) /\
+           (forall x. mem x l2 ==> not (f x)) /\
+           (forall x. mem x l = (mem x l1 || mem x l2)))
+  = match l with
+    | [] -> ()
+    | hd :: tl -> partition_mem f tl
+
+let rec sorted_concat (#a:eqtype)
+                      (f:total_order_t a)
+                      (l1:list a{sorted f l1})
+                      (l2:list a{sorted f l2})
+                      (pivot:a)
+  : Lemma (requires (forall y. mem y l1 ==> not (f pivot y)) /\
+                    (forall y. mem y l2 ==> f pivot y))
+          (ensures sorted f (append l1 (pivot :: l2)))
+  = match l1 with
+    | [] -> ()
+    | hd :: tl -> sorted_concat f tl l2 pivot
+
+let rec append_mem (#t:eqtype)
+                   (l1 l2:list t)
+  : Lemma (ensures (forall a. mem a (append l1 l2) = (mem a l1 || mem a l2)))
+  = match l1 with
+    | [] -> ()
+    | hd::tl -> append_mem tl l2
+
+let rec sort_correct (#a:eqtype) (f:total_order_t a) (l:list a)
+  : Lemma (ensures (
+           let m = sort f l in
+           sorted f m /\
+           (forall i. mem i l = mem i m)))
+          (decreases (length l))
+  = match l with
+    | [] -> ()
+    | pivot :: tl ->
+      let hi, lo  = partition (f pivot) tl in
+      sort_correct f hi;
+      sort_correct f lo;
+      partition_mem (f pivot) tl;
+      sorted_concat f (sort f lo) (sort f hi) pivot;
+      append_mem (sort f lo) (pivot :: sort f hi)
+
+let rec sort_intrinsic (#a:eqtype) (f:total_order_t a) (l:list a)
+  : Tot (m:list a {
+                sorted f m /\
+                (forall i. mem i l = mem i m)
+         })
+   (decreases (length l))
+  = match l with
+    | [] -> []
+    | pivot :: tl ->
+      let hi, lo  = partition (f pivot) tl in
+      partition_mem (f pivot) tl;
+      sorted_concat f (sort_intrinsic f lo) (sort_intrinsic f hi) pivot;
+      append_mem (sort_intrinsic f lo) (pivot :: sort_intrinsic f hi);
+      append (sort_intrinsic f lo) (pivot :: sort_intrinsic f hi)
